Fixes & 2nd property proved

.HOLMK/degChainScript.sml.d
@@ -1,0 +1,1 @@
+degChainScript.uo: /root/HOL/sigobj/IndDefLib.uo /root/HOL/sigobj/ParseExtras.uo /root/HOL/sigobj/TotalDefn.uo /root/cakeml/basis/basis.uo /root/HOL/sigobj/bossLib.uo degTypesTheory.uo /root/HOL/sigobj/listTheory.uo /root/cakeml/translator/monadic/ml_monad_translator_interfaceLib.uo /root/cakeml/misc/preamble.uo /root/HOL/sigobj/stringTheory.uo /root/HOL/sigobj/wordsTheory.uo 
