degPropertiesScript.sml
@@ -1,0 +1,241 @@
+(*START ------------------------------------------------------------------------- *)
+open preamble
+open basis
+open ml_monad_translator_interfaceLib
+
+open stringTheory
+open wordsTheory
+open listTheory
+open degTypesTheory
+open degTheory
+
+val _ = new_theory "degProperties";
+val _ = translation_extends "basisProg";
+val _ = ParseExtras.temp_tight_equality ();
+
+(*CONSTS ------------------------------------------------------------------------ *)
+val const_defs = [
+  (* Errors: *)
+  Define `WRN_PARAMS = "Wrong params"`,
+  Define `RequiredParamIsMissing = "Monadic_EL extract error, some parameter is missing"`,
+  Define `RequiredParamValueMissing = "Type conversion error, some parameter type is incorrect"`,
+  Define `ServersDoNotContainSenderPubKey = "Couldn't find the server that contains sender"`,
+  Define `ServersListIsEmpty = "Servers list is empty"`,
+  Define `VotingIsNotInProgress = "Voting is not in progress (has already finished or not yet started)"`,
+  Define `VotingAlreadyStarted = "Voting has already started"`,
+  Define `SenderIsNotVotingRegistrator = "Sender is not the voting registrator"`,
+  Define `StartDateAlreadyInStateError = "Start date already in state"`,
+  Define `SenderIsNotBlindSigIssueRegistrator = "Sender is not the blind sig issue registrator"`,
+  Define `EmptyStartDateError = "Start date must be in state before operation starts"`,
+  Define `StartDateHasNotComeYet = "Start date has not come yet"`,
+  Define `BlindSigIsNotEqual = "Existing 'blindSig' value is not equal to new value"`, 
+  Define `RevoteIsBlockedError = "Revote is blocked"`,
+  Define `VotingIsNotYetFinished= "Voting is not yet finished (is in progress or not yet started)"`,
+  Define `InvalidCommissionSecretKey = "Commission secret key doesn't match with the commission key from the state"`
+];
+
+(* BEGIN tactics*)
+fun dummy_tac q : tactic
+    = all_tac
+
+fun lambda_comb (COMB pt) = pt
+  | lambda_comb _ = raise Fail "not a lambda COMB"
+
+fun lambdagetpair (COMB pt) = pt
+  | lambdagetpair (LAMB pt) = pt
+  | lambdagetpair _ = raise Fail "wrong constructor"
+
+fun term_by_bin ([]:int list) (t:term) : term = t
+  | term_by_bin (he::ta) t =
+    (let
+      val p = t |> dest_term |> lambdagetpair
+      val st = (if he=0 then (fst p) else (snd p))
+    in
+      term_by_bin ta st
+    end)
+
+(* GET SUBTERM TACTICS *)
+
+(* redundant! it is similar to "strip_comb" function, but works when term con *)
+(*see also strip_fun for types*)
+fun term_as_list te : term list =
+    (term_as_list (rator te)) @ [(rand te)] handle _ => [te]
+
+fun list_as_term li : term = List.foldl (mk_comb o swap) (hd li) (tl li)
+
+val get_head = hd o term_as_list
+val get_args = tl o term_as_list
+
+(* otherwise "val gener:term = ``COND``" gives <<HOL message: inventing new type variable names: 'a>> *)
+fun fst_subterm_matches gener s1 s2 w =
+     let
+       val l = term_as_list w
+       val insta = (el 1 l)
+       val sub = (match_term gener insta)
+         handle _ => raise ERR s1 s2
+     in
+       w
+     end
+
+val gener_ALL : term = ``(!) : (α -> bool) -> bool``
+val checkALL : term -> term = fst_subterm_matches gener_ALL "checkALL" "Not a FORALL term"
+
+val gener_EX : term = ``(?) : (α -> bool) -> bool``
+val checkEX : term -> term = fst_subterm_matches gener_EX "checkEX" "Not an EX term"
+
+val gener_NEG : term = ``(~) : bool -> bool``
+val checkNEG : term -> term = fst_subterm_matches gener_NEG "checkNEG" "Not a NEG term"
+
+val gener_IF : term = ``COND : bool -> α -> α -> α``
+val checkIF : term -> term = fst_subterm_matches gener_IF "checkIF" "Not an IF term"
+
+val gener_EQ : term = ``(=) : α -> α -> bool``
+val checkEQ : term -> term = fst_subterm_matches gener_EQ "checkEQ" "Not an EQ term"
+
+val Cases_on_term: term -> tactic
+     = fn (te : term) => (Cases_on ([ANTIQUOTE te]) >> simp []) : tactic
+
+val get_first_arg  = (el 1) o get_args
+val get_second_arg = (el 2) o get_args
+
+(** Functions for the term destruction **)
+
+fun term_by_num [] t = t
+  | term_by_num (he::ta) t =
+      term_by_num ta (el he $ term_as_list $ t)
+
+(** Functions for the explicit term destruction **)
+
+(* ∀ *)
+val get_forall_body : term -> term
+   = term_by_bin [1,1] o checkALL
+
+(* ∃ *)
+val get_exists_body : term -> term
+   = term_by_bin [1,1] o checkEX
+
+(* get left subterm of equality *)
+val get_eq_left : term -> term
+  = term_by_num [2] o checkEQ
+
+(* get right subterm of equality *)
+val get_eq_right : term -> term
+  = term_by_num [3] o checkEQ
+
+(* get neg's arg *)
+val get_neg : term -> term
+  = term_by_num [2] o checkNEG
+
+(* get IF's condition *)
+val get_if_cond : term -> term
+  = term_by_num [2] o checkIF
+
+val get_cond_term = get_if_cond
+(* see HOL/src/portbleML/Portable.sml *)
+val to_quotation : term -> term quotation
+  = single o ANTIQUOTE
+
+(* get the conclusion of the goal *)
+val get_concl : goal -> term = snd
+
+(* get ==>'s antecedent *)
+val get_antecedent : term -> term
+  = term_by_num [2] (* o checkIMP  TODO! "($==>:bool=>bool=>bool)" *)
+
+(* Using something obtained from the goal as the argument
+   to a function that creates a tactic.
+
+Use cases:
+1) for debug
+  use_goal (print_term o get_neg o get_if_cond o get_eq_left o get_exists_body o get_concl) dummy_tac >>
+2) for reasoning:
+  use_goal (to_quotation o get_neg o get_if_cond o get_eq_left o get_exists_body o get_concl) Cases_on >>
+*)
+
+fun use_goal (obt:goal->'a) (tacf:'a->tactic) : tactic
+    = (fn x as (asl, w) => tacf (obt x) x)
+
+fun print_endline x = print (x ^ "\n")
+val print_term = print_endline o term_to_string
+(* END tactics *)
+
+(* Tactic GET CASE ARGUMENT *)
+val get_case_arg = get_first_arg
+
+val if_inside_casestmnt_tac : tactic =
+ ((fn x => (Cases_on_term o get_first_arg o get_first_arg o snd) x x):tactic)
+
+val addErr_inside_casestmnt_tac : tactic =
+ ((fn x => (Cases_on_term o get_second_arg o get_first_arg o snd) x x):tactic)
+
+fun USE_LAST_HYP (fu:term->tactic) : tactic =
+  (fn x as (asl:term list, w:term) =>
+  (case asl of
+   he :: ta => fu he
+   | _ => raise ERR "USE_LAST_HYP" "there are no hypotheses"
+  ) x)
+
+val FOR_ALL_HYP = REPEAT o USE_LAST_HYP
+
+val UNDISCH_LAST = USE_LAST_HYP UNDISCH_TAC
+
+val UNDISCH_ALL = FOR_ALL_HYP UNDISCH_TAC
+
+val SYM_TAC : tactic = irule EQ_SYM
+
+
+Theorem results_status_error:
+∀ state. ∀  params.   
+(results params state  = fail WRN_PARAMS state) ⇔ (¬(check_types params [TypeNumList]))
+Proof
+  rw []>>
+  simp [results_def]>>
+  simp [ml_monadBaseTheory.st_ex_bind_def] >>
+  simp [ml_monadBaseTheory.st_ex_return_def] >>
+  simp [boolTheory.FUN_EQ_THM] >>
+  simp [get_state_def] >>
+  simp [ml_monadBaseTheory.st_ex_ignore_bind_def] >>
+  simp [assert_def] >>
+  simp [raise_Fail_def, check_types_def]>>
+  rw[]>>EVAL_TAC>>UNDISCH_ALL>>rw[]>>
+  EVAL_TAC >> every_case_tac >>
+  fs [ml_monadBaseTheory.st_ex_bind_def] >>
+  fs [ml_monadBaseTheory.st_ex_return_def] >>
+  fs [boolTheory.FUN_EQ_THM] >>
+  fs [get_state_def] >>
+  fs [ml_monadBaseTheory.st_ex_ignore_bind_def] >>
+  fs [assert_def] >>
+  fs [raise_Fail_def, check_types_def]>>
+  rw[]>>EVAL_TAC>>UNDISCH_ALL>>rw[]
+QED
+
+Theorem results_status_error:
+∀ state. ∀  params.
+(results params state  = fail VotingIsNotYetFinished state) ⇔ 
+(check_types params [TypeNumList] ∧
+∃ l. params = [SCNumList l] ∧
+find_entity state.servers state.context.msg_sender ≠ NONE ∧
+¬(state.votingBase.status = Completed))
+Proof  
+  rw []>>
+  simp [results_def]>>
+  simp [ml_monadBaseTheory.st_ex_bind_def] >>
+  simp [ml_monadBaseTheory.st_ex_return_def] >>
+  simp [boolTheory.FUN_EQ_THM] >>
+  simp [get_state_def] >>
+  simp [ml_monadBaseTheory.st_ex_ignore_bind_def] >>
+  simp [assert_def] >>
+  simp [raise_Fail_def, check_types_def]>>
+  rw[]>>EVAL_TAC>>UNDISCH_ALL>>rw[]>>
+  EVAL_TAC >>every_case_tac >>
+  fs [ml_monadBaseTheory.st_ex_bind_def] >>
+  fs [ml_monadBaseTheory.st_ex_return_def] >>
+  fs [boolTheory.FUN_EQ_THM] >>
+  fs [get_state_def] >>
+  fs [ml_monadBaseTheory.st_ex_ignore_bind_def] >>
+  fs [assert_def] >>
+  fs [raise_Fail_def, check_types_def]>>
+  rw[]>>EVAL_TAC>>UNDISCH_ALL>>rw[]
+QED
+
+val _ = export_theory();
